finish universal property proofs

Semantics/Dynamic/Bool.v
@@ -11,6 +11,7 @@ From ExtensibleCompiler.Theory Require Import Eval.
 From ExtensibleCompiler.Theory Require Import Functor.
 From ExtensibleCompiler.Theory Require Import IndexedAlgebra.
 From ExtensibleCompiler.Theory Require Import IndexedFunctor.
+From ExtensibleCompiler.Theory Require Import IndexedSubFunctor.
 From ExtensibleCompiler.Theory Require Import ProofAlgebra.
 From ExtensibleCompiler.Theory Require Import ProgramAlgebra.
 From ExtensibleCompiler.Theory Require Import SubFunctor.
@@ -26,20 +27,20 @@ Definition eval__Bool
   : forall {T}, MixinAlgebra Bool T (EvalResult V)
   := fun _ rec '(MkBool b) env => boolean b.
 
-Global Instance EvalAlgebra__Bool
+Global Instance Eval__Bool
        {V} `{FunctorLaws V}
        `{! V supports Bool}
   : forall {T}, ProgramAlgebra Eval Bool T (EvalResult V)
   := fun _ => {| programAlgebra := eval__Bool; |}.
 
-Inductive Eval__Bool {L V}
-          `{FunctorLaws L} `{FunctorLaws V}
-          `{! L supports Bool}
+Inductive EvalP__Bool {E V}
+          `{FunctorLaws E} `{FunctorLaws V}
+          `{! E supports Bool}
           `{! V supports Bool}
-          (Eval_E : (WellFormedValue L * WellFormedValue V) -> Prop)
-  : (WellFormedValue L * WellFormedValue V) -> Prop
+          (EvalP__E : (WellFormedValue E * WellFormedValue V) -> Prop)
+  : (WellFormedValue E * WellFormedValue V) -> Prop
   :=
-  | BoolValue : forall b, Eval__Bool Eval_E (boolean b, boolean b)
+  | BoolValue : forall b, EvalP__Bool EvalP__E (boolean b, boolean b)
 .
 
 Inductive WellTyped__Bool
@@ -51,7 +52,21 @@ Inductive WellTyped__Bool
 | WellTyped__boolean : forall t e b,
     proj1_sig e = boolean__F b ->
     proj1_sig t = boolType ->
-    WellTyped__Bool WT {| type := t; expr := e; |}.
+    WellTyped__Bool WT {| type := t; expr := e; |}
+.
+
+Global Instance IndexedFunctor_WellTyped__Bool
+       {T V}
+       `{FunctorLaws T} `{FunctorLaws V}
+       `{! T supports BoolType}
+       `{! V supports Bool}
+  : IndexedFunctor (TypedExpr T V) WellTyped__Bool.
+Proof.
+  constructor.
+  move => A B i IH [] [t UP__t] [e UP__e] b /= => Eq__e Eq__t.
+  move : Eq__t Eq__e UP__t UP__e => -> -> => UP__t UP__e.
+  econstructor => //.
+Qed.
 
 Definition SoundnessStatement__Bool
            {T E V}
@@ -70,18 +85,32 @@ Definition SoundnessStatement__Bool
     ).
 
 Global Instance EvalSoundness__Bool
-       {T E V}
-       `{FunctorLaws T} `{FunctorLaws E} `{FunctorLaws V}
-       `{! E supports Bool} `{! WellFormedSubFunctor Bool E}
+
+       {T}
+       `{FunctorLaws T}
        `{! T supports BoolType}
+
+       {E}
+       `{FunctorLaws E}
+       `{! E supports Bool}
+       `{! WellFormedSubFunctor Bool E}
+
+       {V}
+       `{FunctorLaws V}
        `{! V supports Bool}
+
        (WT : (TypedExpr T V -> Prop) -> TypedExpr T V -> Prop)
+       `(IndexedFunctor (TypedExpr T V) WT)
+       `((WellTyped__Bool <= WT)%IndexedSubFunctor)
+
        `{Eval__E   : forall {R}, ProgramAlgebra Eval   E R (EvalResult   V)}
-       `{! forall {R}, WellFormedProgramAlgebra EvalAlgebra__Bool Eval__E (T := R)}
+       `{! forall {R}, WellFormedProgramAlgebra Eval__Bool Eval__E (T := R)}
+       (recEval   : UniversalPropertyF E -> EvalResult   V)
+
        `{TypeOf__E : forall {R}, ProgramAlgebra TypeOf E R (TypeOfResult T)}
        `{! forall {R}, WellFormedProgramAlgebra TypeOf__Bool TypeOf__E (T := R)}
-       (recEval   : UniversalPropertyF E -> EvalResult   V)
        (recTypeOf : UniversalPropertyF E -> TypeOfResult T)
+
   : ProofAlgebra Bool (sig (UniversalPropertyP2 (SoundnessStatement__Bool WT recEval recTypeOf))).
 Proof.
   constructor.
@@ -100,13 +129,10 @@ Proof.
     rewrite / programAlgebra'.
     rewrite wellFormedProgramAlgebra.
     rewrite wellFormedProgramAlgebra.
-    move => IH tau.
-    rewrite / programAlgebra.
-    rewrite / EvalAlgebra__Bool / eval__Bool.
-    rewrite / TypeOf__Bool / typeOf__Bool.
-    move => [] <-.
-    rewrite / WellTyped.
-
-    admit.
+    move => IH tau TY.
+    apply (iInject (F := WellTyped__Bool)) => /=.
+    econstructor => //.
+    move : TY => /=.
+    move => [] <- //.
   }
-Admitted.
+Qed.
